QuantSepCon.thy
@@ -1072,14 +1072,14 @@ text \<open>Allowing a second operation on the measuring type.\<close>
 
 locale quant_sep_con_oper2 =  quant_sep_con oper neutr divide
   for  
-      oper :: "'b::{complete_lattice} \<Rightarrow> 'b \<Rightarrow> 'b"  (infixl "\<^bold>*" 70)
+    oper :: "'b::{complete_lattice} \<Rightarrow> 'b \<Rightarrow> 'b"  (infixl "\<^bold>*" 70)
     and neutr :: "'b" ("\<^bold>1") 
-    and  divide :: "'b \<Rightarrow> 'b \<Rightarrow> 'b"  (infixl "\<^bold>div" 70) +
+    and divide :: "'b \<Rightarrow> 'b \<Rightarrow> 'b"  (infixl "\<^bold>div" 70) +
   fixes
-      oper2 :: "'b \<Rightarrow> 'b \<Rightarrow> 'b" (infixl "\<^bold>+" 65)
-    assumes
-      plusmal_distrib[algebra_simps]: "\<And>a b c. a \<^bold>* (b \<^bold>+ c) = a \<^bold>* b \<^bold>+ a \<^bold>* c"
-      and oper2_mono: "\<And>a b c d. a \<le> b \<Longrightarrow> c \<le> d \<Longrightarrow> a \<^bold>+ c \<le> b \<^bold>+ d"
+    oper2 :: "'b \<Rightarrow> 'b \<Rightarrow> 'b" (infixl "\<^bold>+" 65)
+  assumes
+    plusmal_distrib[algebra_simps]: "\<And>a b c. a \<^bold>* (b \<^bold>+ c) = a \<^bold>* b \<^bold>+ a \<^bold>* c"
+    and oper2_mono: "\<And>a b c d. a \<le> b \<Longrightarrow> c \<le> d \<Longrightarrow> a \<^bold>+ c \<le> b \<^bold>+ d"
 begin
 
 
@@ -1092,9 +1092,9 @@ begin
 
 lemma theorem_3_6_general2: 
   fixes
-      P :: "_ \<Rightarrow> 'b"  
+    P :: "_ \<Rightarrow> 'b"  
   shows
-  "((P **q (\<lambda>h. Q h \<^bold>+ R h)) h) \<le> ((P **q Q) h) \<^bold>+ ((P **q R) h)"
+    "((P **q (\<lambda>h. Q h \<^bold>+ R h)) h) \<le> ((P **q Q) h) \<^bold>+ ((P **q R) h)"
 proof -
   have "(P **q (\<lambda>h. Q h \<^bold>+ R h)) h = (SUP (x,y):{(x,y)|x y. h = x + y \<and> x ## y}. (P x \<^bold>* Q y) \<^bold>+ (P x \<^bold>* R y) )"
     unfolding sep_conj_q_alt  by (simp add: plusmal_distrib) 
@@ -1111,7 +1111,7 @@ qed
 
 end
 end
- 
+
 
 
 end
